TrGroupFun.v
@@ -1,0 +1,242 @@
+(**
+
+This file describes grouping transformation relations as functions.
+
+Author: Ramon Fernandez I Mir and Arthur Charguéraud.
+
+License: MIT.
+
+*)
+
+Set Implicit Arguments.
+Require Export Semantics LibSet LibMap TLCbuffer TrGroup.
+
+
+(* ---------------------------------------------------------------------- *)
+(** Hints *)
+
+(* TODO: Factor this out. *)
+Lemma index_of_index_length : forall A (l' l : list A) i,
+  index l' i ->
+  length l' = length l ->
+  index l i.
+Proof.
+  intros. rewrite index_eq_index_length in *.
+  applys* index_of_index_length'.
+Qed.
+
+Hint Resolve index_of_index_length.
+
+Hint Constructors red.
+Hint Constructors tr_trm tr_val tr_accesses tr_state tr_stack.
+Hint Constructors read_accesses write_accesses.
+
+
+(* ---------------------------------------------------------------------- *)
+(** Functionality of the relations *)
+
+Theorem functional_tr_accesses : forall gt π π1 π2,
+  tr_accesses gt π π1 ->
+  tr_accesses gt π π2 ->
+    π1 = π2.
+Proof.
+  introv H1 H2. gen π2. induction H1; intros;
+  inverts_head tr_accesses; repeat fequals*;
+  inverts_head Logic.or; repeat fequals*.
+Qed. 
+
+Theorem functional_tr_val : forall gt v v1 v2,
+  tr_val gt v v1 ->
+  tr_val gt v v2 ->
+  v1 = v2.
+Proof using.
+  introv H1 H2. gen v2. induction H1; intros;
+  inverts_head tr_val; fequals*.
+  { applys* functional_tr_accesses. }
+  { applys* eq_of_extens. math. }
+  { applys read_extens. 
+    { inverts_head make_group_tr'. congruence. }
+    { introv Hin. tests C: (i = fg).
+      { inverts_head make_group_tr'.
+        asserts_rewrite~ (s'0[fg0] = val_struct Tsg0 sg0).
+        asserts_rewrite~ (s'[fg0] = val_struct Tsg0 sg).
+        fequals. applys~ read_extens. introv Hk. 
+        asserts_rewrite* (dom sg = dom sg0) in *. }
+      { inverts_head make_group_tr'.
+        asserts_rewrite~ (dom s' = dom s \- dom sg \u '{fg0}) in Hin.
+        inverts Hin as Hin; tryfalse. inverts Hin as Hin Hnotin.
+        asserts_rewrite* (dom sg = dom sg0) in *. } } }
+  { subst. simpls. contradiction. }
+  { applys read_extens.
+    { congruence. }
+    { introv Hin. 
+      asserts_rewrite* (dom s' = dom s) in *. } }
+Qed.
+
+Theorem functional_tr_trm : forall gt t t1 t2,
+  tr_trm gt t t1 ->
+  tr_trm gt t t2 ->
+  t1 = t2.
+Proof.
+  introv H1 H2. gen t2. induction H1; intros;
+  try solve [ inverts H2 ; try subst ; repeat fequals* ].
+  { inverts H2. fequals. applys* functional_tr_val. }
+  { inverts_head tr_trm; subst. 
+    { repeat fequals~. }
+    { inverts_head Logic.or; tryfalse. } 
+    { unfolds is_prim_struct_access. contradiction. } }
+  { inverts_head tr_trm; subst.
+    { inverts_head Logic.or; tryfalse. }
+    { repeat fequals~. } 
+    { unfolds is_prim_struct_access. contradiction. } }
+  { inverts_head tr_trm; 
+    try solve [ unfolds is_prim_struct_access ; contradiction ].
+    repeat fequals~. }
+Qed.
+
+Theorem functional_tr_stack_item : forall gt i i1 i2,
+  tr_stack_item gt i i1 ->
+  tr_stack_item gt i i2 ->
+  i1 = i2.
+Proof.
+  introv Hi1 Hi2. 
+  inverts Hi1 as H. inverts Hi2 as H'. 
+  forwards*: functional_tr_val H H'.
+Qed.
+
+Theorem functional_tr_stack : forall gt S S1 S2,
+  tr_stack gt S S1 ->
+  tr_stack gt S S2 ->
+  S1 = S2.
+Proof.
+  introv HS1 HS2. inverts HS1 as HS1. inverts HS2 as HS2. 
+  gen S2. induction HS1; intros.
+  { inverts~ HS2. }
+  { inverts HS2 as HSy0 HS1'. fequals.
+    { forwards*: functional_tr_stack_item H HSy0. }
+    { applys~ IHHS1. } }
+Qed.
+
+Theorem functional_tr_state : forall gt m m1 m2,
+  tr_state gt m m1 ->
+  tr_state gt m m2 ->
+  m1 = m2.
+Proof.
+  introv Hm1 Hm2. 
+  inverts Hm1 as HD1 Htr1. inverts Hm2 as HD2 Htr2.
+  applys read_extens.
+  { unfolds state. congruence. }
+  { introv Hi. rewrite HD1 in *. 
+    forwards Hm1i: Htr1 Hi. forwards Hm2i: Htr2 Hi.
+    forwards~: functional_tr_val Hm1i Hm2i. }
+Qed.
+
+
+(* ---------------------------------------------------------------------- *)
+(** Explicit definitions *)
+
+Fixpoint fun_tr_accesses (gt:group_tr) (π:accesses) : accesses :=
+  let aux := fun_tr_accesses gt in
+  match π with
+  | nil => nil
+  | ((access_array i)::π') => ((access_array i)::(aux π'))
+  | ((access_field T f)::π') => 
+      if isTrue(T = group_tr_struct_name gt) then
+        if isTrue(f \in group_tr_fields gt) then
+          let Tg := group_tr_new_struct_name gt in
+          let fg := group_tr_new_struct_field gt in
+          ((access_field T fg)::(access_field Tg f)::(aux π'))
+        else
+          ((access_field T f)::(aux π'))
+      else
+        ((access_field T f)::(aux π'))
+  end.
+
+Fixpoint fun_tr_val_depth (depth:nat) (gt:group_tr) (v:val) : val :=
+  match depth with
+    | O => v
+    | S n =>
+      let aux := fun_tr_val_depth n gt in
+      match v with
+      | val_error => val_error
+      | val_uninitialized => val_uninitialized
+      | val_unit => val_unit
+      | val_bool b => val_bool b
+      | val_int i => val_int i
+      | val_double d => val_double d
+      | val_abstract_ptr l π => val_abstract_ptr l (fun_tr_accesses gt π)
+      | val_array nil => val_array nil
+      | val_array vs => (val_array (LibList.map aux vs)) 
+      | val_struct T s =>
+          let m : monoid_op (map field val) := monoid_make (fun a b => a \u b) \{} in
+          let g : field -> val -> map field val := fun f v => (\{})[f:=(aux v)] in
+          if isTrue(T=group_tr_struct_name gt) then
+            let Tg := group_tr_new_struct_name gt in
+            let fg := group_tr_new_struct_field gt in
+            let fs := group_tr_fields gt in
+            let s' := fold m g s in
+            let g1' : field -> val -> map field val := 
+              fun f v => if (isTrue(f \in fs)) then (\{}) else (\{})[f:=v] in
+            let g2' : field -> val -> map field val := 
+              fun f v => if (isTrue(f \in fs)) then (\{})[f:=v] else (\{}) in
+            let s1' := fold m g1' s in
+            let s2' := fold m g2' s in
+            val_struct T (s1'[fg:=(val_struct Tg s2')])
+          else
+            val_struct T (fold m g s)
+      end
+   end.
+
+
+(* ---------------------------------------------------------------------- *)
+(** Lemmas outline *)
+
+Lemma fixpoint_fun_tr_val : forall gt n v,
+  fun_tr_val_depth n gt v = fun_tr_val_depth (S n) gt v ->
+  tr_val gt v (fun_tr_val_depth n gt v).
+Proof.
+Admitted.
+
+Lemma depth_fun_tr_val : forall gt v,
+  exists n, tr_val gt v (fun_tr_val_depth n gt v).
+Proof.
+Admitted.
+
+Lemma total_tr_accesses : forall gt π,
+  exists π', tr_accesses gt π π'.
+Proof.
+  induction π; eauto. destruct a.  
+  { inverts IHπ; exists __. constructors*.  }
+  { tests: (t = group_tr_struct_name gt).
+    { tests: (f \in group_tr_fields gt).
+      { inverts IHπ; exists __. applys* tr_accesses_field_group. }
+      { inverts IHπ; exists __. applys* tr_accesses_field_other. } }
+    { inverts IHπ; exists __. applys* tr_accesses_field_other. } }
+Qed.
+
+Lemma total_tr_val : forall gt v,
+  exists v', tr_val gt v v'.
+Proof.
+  intros. forwards* (n&H): depth_fun_tr_val gt v.
+Qed.
+
+(*Lemma tr_array : forall gt (a:list val),
+  exists a', 
+        length a' = length a
+    /\  (forall i, 
+          index a' i -> 
+          tr_val gt a[i] a'[i]).
+Proof.
+  induction a.
+  { exists __. rewrite length_nil in *. splits~. introv Hi.
+    inverts Hi. rewrite LibList.length_nil in *. math. }
+  { inverts IHa as (IHl&IHx). forwards (v'&Hv'): total_tr_val gt a.
+    exists (v'::x). splits.
+    { repeat rewrite length_cons. fequals. }
+    { introv Hi. tests: (i = 0).
+      { repeat rewrite~ read_zero. }
+      { repeat rewrite read_cons_case. case_if*. 
+        inverts Hi. forwards~: IHx (i - 1).
+        applys int_index_prove. math.  
+        rewrite LibList.length_cons in *. math. } } }
+Qed.*)
