TrTiling.v
@@ -1,0 +1,220 @@
+(**
+
+This file describes transformations of the layout of records and arrays.
+
+Author: Ramon Fernandez I Mir and Arthur Charguéraud.
+
+License: MIT.
+
+*)
+
+Set Implicit Arguments.
+Require Export Semantics LibSet LibMap TLCbuffer.
+
+
+(* ********************************************************************** *)
+(* * Definition of the transformation *)
+
+(** Grouping transformation. Specified by:
+    - The name of the struct to be modified.
+    - The set of fields to be grouped.
+    - The name of the new struct that will hold the fields to be grouped.
+    - The name of the field in the new struct that will have as type
+      the new struct. *)
+
+Record group_tr := make_group_tr {
+  group_tr_struct_name : typvar;
+  group_tr_fields : set field;
+  group_tr_new_struct_name : typvar;
+  group_tr_new_struct_field : field
+}.
+
+Notation make_group_tr' := make_group_tr.
+
+(** Transformation of paths: π ~ |π| *)
+
+Inductive tr_accesses (gt:group_tr) : accesses -> accesses -> Prop :=
+  | tr_accesses_nil :
+      tr_accesses gt nil nil
+  | tr_accesses_array : forall π π' i,
+      tr_accesses gt π π' ->
+      tr_accesses gt ((access_array i)::π) ((access_array i)::π')
+  | tr_accesses_field_group : forall π π' f fg Ts Tsg,
+      tr_accesses gt π π' ->
+      Ts = group_tr_struct_name gt ->
+      Tsg = group_tr_new_struct_name gt ->
+      f \in (group_tr_fields gt) ->
+      fg = group_tr_new_struct_field gt ->
+      tr_accesses gt ((access_field Ts f)::π) ((access_field Ts fg)::(access_field Tsg f)::π')
+  | tr_accesses_field_other : forall T Ts π π' f,
+      tr_accesses gt π π' ->
+      Ts = group_tr_struct_name gt ->
+      (T <> Ts \/ f \notin (group_tr_fields gt)) ->
+      tr_accesses gt ((access_field T f)::π) ((access_field T f)::π').
+
+(** Transformation of values: v ~ |v| *)
+
+Inductive tr_val (gt:group_tr) : val -> val -> Prop :=
+  | tr_val_error :
+      tr_val gt val_error val_error
+  | tr_val_uninitialized :
+      tr_val gt val_uninitialized val_uninitialized
+  | tr_val_unit :
+      tr_val gt val_unit val_unit
+  | tr_val_bool : forall b,
+      tr_val gt (val_bool b) (val_bool b)
+  | tr_val_int : forall i,
+      tr_val gt (val_int i) (val_int i)
+  | tr_val_double : forall d,
+      tr_val gt (val_double d) (val_double d)
+  | tr_val_abstract_ptr : forall l π π',
+      tr_accesses gt π π' ->
+      tr_val gt (val_abstract_ptr l π) (val_abstract_ptr l π')
+  | tr_val_array : forall a a',
+      length a = length a' ->
+      (forall i,
+        index a i ->
+        tr_val gt a[i] a'[i]) ->
+      tr_val gt (val_array a) (val_array a')
+  | tr_val_struct_group : forall Ts Tsg s s' fg fs sg,
+      gt = make_group_tr Ts fs Tsg fg ->
+      fs \c dom s ->
+      fg \notindom s ->
+      dom s' = (dom s \- fs) \u \{fg} ->
+      dom sg = fs ->
+      (forall f,
+        f \indom sg ->
+        tr_val gt s[f] sg[f]) ->
+      (forall f,
+        f \notin fs ->
+        f \indom s ->
+        tr_val gt s[f] s'[f]) ->
+      s'[fg] = val_struct Tsg sg ->
+      tr_val gt (val_struct Ts s) (val_struct Ts s')
+  | tr_val_struct_other : forall T s s',
+      T <> group_tr_struct_name gt ->
+      dom s = dom s' ->
+      (forall f,
+        f \indom s ->
+        tr_val gt s[f] s'[f]) ->
+      tr_val gt (val_struct T s) (val_struct T s').
+
+Definition is_prim_struct_access (op:prim) :=
+  match op with
+  | prim_struct_access _ _ => True
+  | _ => False
+  end.
+
+
+(** Transformation of terms: t ~ |t| *)
+
+Inductive tr_trm (gt:group_tr) : trm -> trm -> Prop :=
+  | tr_trm_val : forall v v',
+      tr_val gt v v' ->
+      tr_trm gt (trm_val v) (trm_val v')
+  | tr_trm_var : forall x,
+      tr_trm gt (trm_var x) (trm_var x)
+  | tr_trm_if : forall t1 t2 t3 t1' t2' t3',
+      tr_trm gt t1 t1' ->
+      tr_trm gt t2 t2' ->
+      tr_trm gt t3 t3' ->
+      tr_trm gt (trm_if t1 t2 t3) (trm_if t1' t2' t3')
+  | tr_trm_let : forall x t1 t2 t1' t2',
+      tr_trm gt t1 t1' ->
+      tr_trm gt t2 t2' ->
+      tr_trm gt (trm_let x t1 t2) (trm_let x t1' t2')
+  (* new *)  
+  | tr_trm_new : forall T,
+      tr_trm gt (trm_app (prim_new T) nil) (trm_app (prim_new T) nil)
+  (* Special case: struct access *)
+  | tr_trm_struct_access_x : forall p p' s s_g f f_g a1 a2 r,
+      tr_trm gt p p' ->
+      s = group_tr_struct_name gt ->
+      s_g = group_tr_new_struct_name gt ->
+      f \in (group_tr_fields gt) ->
+      f_g = group_tr_new_struct_field gt ->
+      a1 = prim_struct_access s_g f ->
+      a2 = prim_struct_access s f_g ->
+      r = trm_app a1 ((trm_app a2 (p'::nil))::nil) ->
+      tr_trm gt (trm_app (prim_struct_access s f) (p::nil)) r
+  | tr_trm_struct_access_other : forall s p p' T f r,
+      tr_trm gt p p' ->
+      s = group_tr_struct_name gt ->
+      (T <> s \/ f \notin (group_tr_fields gt)) ->
+      r = (trm_app (prim_struct_access T f) (p'::nil)) ->
+      tr_trm gt (trm_app (prim_struct_access T f) (p::nil)) r
+  (* Args *)
+  | tr_trm_args1 : forall op t1 t1',
+      ~ is_prim_struct_access op ->
+      tr_trm gt t1 t1' ->
+      tr_trm gt (trm_app op (t1::nil)) (trm_app op (t1'::nil))
+  | tr_trm_args2 : forall op t1 t1' t2 t2',
+      tr_trm gt t1 t1' ->
+      tr_trm gt t2 t2' ->
+      tr_trm gt (trm_app op (t1::t2::nil)) (trm_app op (t1'::t2'::nil)).
+
+
+(** Transformation of stacks: S ~ |S| *)
+
+Inductive tr_stack_item (gt:group_tr) : (var * val) -> (var * val) -> Prop :=
+  | tr_stack_item_intro : forall x v v',
+      tr_val gt v v' -> 
+      tr_stack_item gt (x, v) (x, v').
+
+Inductive tr_stack (gt:group_tr) : stack -> stack -> Prop :=
+  | tr_stack_intro : forall S S',
+      LibList.Forall2 (tr_stack_item gt) S S' ->
+      tr_stack gt S S'.
+
+Lemma stack_lookup_tr : forall gt S S' x v,
+  tr_stack gt S S' ->
+  Ctx.lookup x S = Some v -> 
+    exists v', 
+       Ctx.lookup x S' = Some v' 
+    /\ tr_val gt v v'.
+Proof.
+  introv HS Hx. inverts HS as HS. induction HS.
+  { inverts Hx. }
+  { inverts H as Hv. inverts Hx as Hx. case_if in Hx.
+    { inverts Hx. exists v'. splits*. unfolds. case_if*. }
+    { forwards (v''&Hx'&Hv''): IHHS Hx. exists v''.
+      splits*. unfolds. case_if. fold Ctx.lookup. auto. } }
+Qed.
+
+
+(** Transformation of states: m ~ |m| *)
+
+Inductive tr_state (gt:group_tr) : state -> state -> Prop :=
+  | tr_state_intro : forall m m',
+      dom m = dom m' ->
+      (forall l,
+        l \indom m ->
+        tr_val gt m[l] m'[l]) ->
+      tr_state gt m m'.
+
+
+(** Transformation of typdefctxs: C ~ |C| *)
+
+Inductive tr_typdefctx (gt:group_tr) : typdefctx -> typdefctx -> Prop :=
+  | tr_typdefctx_intro : forall Tt fs Tg fg C C',
+      gt = make_group_tr Tt fs Tg fg ->
+      Tt \indom C ->
+      Tg \notindom C ->
+      dom C' = dom C \u \{Tg} ->
+      (forall T,
+        T \indom C ->
+        T <> Tt ->
+        C'[T] = C[T]) ->
+      fs \c dom (C[Tt]) ->
+      fg \notindom (C[Tt]) ->
+      dom (C'[Tt]) = (dom (C[Tt]) \- fs) \u \{fg} ->
+      (forall f,
+        f \indom (C[Tt]) ->
+        f \notin fs ->
+        C'[Tt][f] = C[Tt][f]) ->
+      C'[Tt][fg] = typ_struct Tg ->
+      dom (C'[Tg]) = fs ->
+      (forall f,
+        f \indom (C'[Tg]) ->
+        C'[Tg][f] = C[Tt][f]) ->
+      tr_typdefctx gt C C'.
